

Chapter 1

MathStat Preliminaries

1.1

Wait. Where are we going?

Exponential pdf

If $X \sim \text{Exponential}(\lambda)$, then X has the pdf
 $f(x) = \lambda \exp(-\lambda x) I_{[0, \infty]}(x)$.

Exponential pdf visualized

Sample

A sample of n realization of X , denoted X_1, X_2, \dots, X_n , can be used to approximate the distribution of X .

Histogram for 10 realizations

A histogram of 10 realizations from an Exponential(15.2).

Histogram for 1000 realizations

A histogram of 1000 realizations from an Exponential(15.2).

1.1.1

A very special trick

Approach

We can avoid doing actual integration if we can manipulate the integrand to look more like a pdf, which must integrate to 1 of the range of the random variable.

Example: Determine

$$\int_0^{\infty} 3 \exp(-2x) dx.$$

Special trick (cont)

1.2

Transformations of Random Variables

1.2.1

The discrete case and the binomial distribution

The binomial pmf

$X \sim \text{Binomial}(n, p)$ has the pmf

$$f(x) = P(X = x) = \binom{n}{x} p^x (1 - p)^{n-x} I_{\{0,1,\dots,n\}}(x).$$

Determine the pmf of $Y := n - X$.

1.2.2

The Continuous Case and the Gamma Distribution

Continuous Transformation PDF

Let X be a continuous random variable with pdf $f_X(x)$. Let $Y = g(X)$, where g is invertible and differentiable. Then the pdf for Y is

$$f_Y(y) = f_X(g^{-1}(y)) \left| \frac{d}{dy} g^{-1}(y) \right|.$$

Proof

Proof (cont)

Proof (cont)

Proof (cont)

Example 1.2.2

A continuous random variable $X \sim \text{Gamma}(\alpha, \beta)$ has pdf

$$f_X(x) = \frac{1}{\Gamma(\alpha)} \beta^\alpha x^{\alpha-1} \exp(-\beta x) I_{(0,\infty)}(x).$$

Example 1.2.2 (cont)

Let $Y := cX$ with $c > 0$. Determine the pdf of Y .

Example 1.2.2 (cont)

The shape parameter

The α term is the “shape” parameter of the Gamma distribution.

The kernel (non-constant) part of the pdf of the Gamma distribution is

$$x^{\alpha-1} \exp(-\beta x) I_{(0,\infty)}(x).$$

The shape parameter

The exponential function part is an unscaled exponential density.

- $\exp(-\beta x)$ dominates $x^{\alpha-1}$ for large x .
- For small x , the $x^{\alpha-1}$ term controls the shape.

Shape parameter visualized

The α terms controls the shape of the Gamma distribution.

The Gamma Function

The pdf for the gamma distribution is defined using the **gamma function**, denoted by $\Gamma(\alpha)$.

$$\Gamma(\alpha) = \int_0^{\infty} x^{\alpha-1} \exp(-x) dx.$$

The Gamma Function (cont)

The Gamma Function (cont)

The Gamma Function (cont)

1.3

Bivariate Transformations

Bivariate Transformation PDF

Suppose the X_1 and X_2 are jointly continuous random variables with pdf $f_{X_1, X_2}(x_1, x_2)$. Let $Y_1 = g_1(X_1, X_2)$ and $Y_2 = g_2(X_1, X_2)$. For h_1 and h_2 differentiable, let

$$X_1 = h_1(Y_1, Y_2) \text{ and } X_2 = h_2(Y_1, Y_2).$$

Then

$$f_{Y_1, Y_2}(y_1, y_2) = f_{X_1, X_2}(h_1(y_1, y_2), h_2(y_1, y_2)) |J|,$$

where $|J|$ is the absolute value of the Jacobian.

Bivariate transformation pdf continued

The absolute value of the Jacobian is

$$J = \det \begin{bmatrix} \frac{\partial x_1}{\partial y_1} & \frac{\partial x_1}{\partial y_2} \\ \frac{\partial x_2}{\partial y_1} & \frac{\partial x_2}{\partial y_2} \end{bmatrix}.$$

Example 1.3.1

Let $X_1, X_2 \stackrel{i.i.d.}{\sim} \text{Gamma}(\alpha, \beta)$

Determine the pdf of

$$Y = \frac{X_1}{X_1 + X_2}.$$

Example 1.3.1 (cont)

Example 1.3.1 (cont)

Example 1.3.1 (cont)

Example 1.3.1 (cont)

The Beta Distribution

The continuous random variable $X \sim \text{Beta}(a, b)$ had pdf

$$f(x) = \frac{1}{\mathcal{B}(a, b)} x^{a-1} (1-x)^{b-1} I_{(0,1)}(x),$$

for $a, b > 0$, where

$$\mathcal{B}(a, b) = \int_0^1 x^{a-1} (1-x)^{b-1} dx$$

denotes the **beta function**, which normalizes the kernel of the Beta distribution.

The Beta Distribution (cont)

The Beta distribution is a flexible distribution for modeling a random variable between 0 and 1.

Note: The Uniform(0, 1) distribution is a special case of the Beta distribution with

The Beta Distribution (cont)

The Beta Function

$$\mathcal{B}(a, b) = \frac{\Gamma(a)\Gamma(b)}{\Gamma(a+b)}.$$

Proof:

The Beta Function (cont)

1.4

Minimums and Maximums

Order statistics notation

Let X_1, X_2, \dots, X_n denote a sample of observations. The order statistics are denoted as:

- $X_{(1)} = \min(X_1, X_2, \dots, X_n)$.
- $X_{(2)} =$ 2nd smallest of X_1, X_2, \dots, X_n .
- $X_{(n)} = \max(X_1, X_2, \dots, X_n)$.

1.4.2

The distribution of a minimum by example

Example 1.4.1

Let $X_1, X_2, \dots, X_n \stackrel{i.i.d.}{\sim} \text{Exponential}(\lambda)$. Determine the distribution of $X_{(1)}$.

Example 1.4.1 (cont)

Example 1.4.1 (cont)

Example 1.4.1 (cont)

Example 1.4.1 (cont)

1.4.3

The general distribution of minimums and maximums

Distribution of the minimum

Let X_1, X_2, \dots, X_n be a random sample from a continuous distribution. Determine the distribution of $X_{(1)}$.

Distribution of the minimum (cont)

Distribution of the minimum (cont)

Distribution of the minimum (cont)

PDF for a minimum

Let X_1, X_2, \dots, X_n be a random sample from a continuous distribution with pdf f and cdf F .

The pdf for $X_{(1)}$ is

$$f_{X_{(1)}} = n[1 - F(x)]^{n-1} f(x).$$

Distribution of the maximum

Let X_1, X_2, \dots, X_n be a random sample from a continuous distribution. Determine the distribution of $X_{(n)}$.

Distribution of the maximum (cont)

Distribution of the maximum (cont)

Distribution of the maximum (cont)

PDF for a maximum

Let X_1, X_2, \dots, X_n be a random sample from a continuous distribution with pdf f and cdf F .

The pdf for $X_{(n)}$ is

$$f_{X_{(n)}} = n[F(x)]^{n-1} f(x).$$

1.5

Moment Generating Functions (mgfs)

Definition of the mgf

The moment generating function (mgf) of a random variable X is $M_X(t) = E[e^{tX}]$.

Uses of mgfs

Mgfs are often useful in two settings:

1. Determining the distribution of a transformation of 1 or more random variables (particularly the sum of n i.i.d. random variables.)
2. Determine the “moments” of a random variable, i.e., $E(X)$, $E(X^2)$, $E(X^3)$, \dots

1.5.1

The expectation of a function X

Example 1.5.1

Suppose the random variable X has the following distribution.

x	-1	0	1
<hr/>			
$f(x)$	4/12	3/12	5/12

Determine $E(X^2)$.

Example 1.5.1 (cont)

Example 1.5.1 (cont)

Law of the Unconscious Statistician

If X is a discrete random variable, then

$$E[g(X)] = \sum_x g(x) f_X(x),$$

where $f_X(x)$ is the pmf of X .

If X is a continuous random variable, then

$$E[g(X)] = \int_{-\infty}^{\infty} g(x) f_X(x) dx,$$

where $f_X(x)$ is the pdf of X .

Proof (specific case)

Proof (specific case)

Proof (specific case)

Proof (specific case)

1.5.2

Finding mgfs and the Poisson distribution

The Poisson distribution

A discrete random variable $X \sim \text{Poisson}(\lambda)$ if it has the pmf

$$f_X(x) = \frac{e^{-\lambda} \lambda^x}{x!} I_{\{0,1,2,\dots\}}(x).$$

Poisson interpretation

A Poisson random variable can be thought of as the number of arrivals observed in a fixed amount of time where:

1. The mean time between arrivals is constant.
2. The number of arrivals in non-overlapping time periods are independent.

Example 1.5.2

Determine the mgf for the Poisson distribution

Example 1.5.2 (cont)

Example 1.5.2 (cont)

Example 1.5.3

Suppose that $X \sim \text{Exponential}(\lambda)$. Determine the mgf of X .

Example 1.5.3 (cont)

Example 1.5.3 (cont)

Example 1.5.4

Suppose that $X \sim N(\mu, \sigma^2)$ with pdf

$$f_X(x) = \frac{1}{\sigma\sqrt{2\pi}} \exp\left[-\frac{1}{2\sigma^2}(x - \mu)^2\right].$$

Determine the mgf of X .

Example 1.5.4 (cont)

Example 1.5.4 (cont)

Example 1.5.4 (cont)

1.5.3

Finding moments

Defining moments

The **moments** of a random variable X are expectations of the form $E(X^k)$ for $k = 1, 2, 3, \dots$

Computing moments

The k th moment of a random variable X can be computed as $M_X^{(k)}(0)$, where $M_X^{(k)}(0)$ is the k th derivative of the mgf of X evaluated at zero.

Mgf moment proof

Mgf moment proof (cont)

Mgf moment proof (cont)

Example 1.5.5

Determine the mean and variance of the $\text{Poisson}(\lambda)$ distribution.

Example 1.5.5 (cont)

Example 1.5.5 (cont)

1.5.4

The mgf uniquely determines a distribution

The DNA of the mgf

The mgf of a random variable uniquely determines its distribution.

Example: If we find the mgf of a random variable X is $\exp[15(e^t - 1)]$, then $X \sim \text{Poisson}(15)$ since it matches the mgf of a Poisson random variable with $\lambda = 15$.

1.5.6

Sums of iid random variables

Mgf of sum of independent r.v.s

Let X_1, X_2, \dots, X_n be independent random variables. The mgf of

$$Y := \sum_{i=1}^n X_i$$

is

$$M_Y(t) = \prod_{i=1}^n M_{X_i}(t).$$

Proof

Proof (cont)

Proof (cont)

Mgf of sum of i.i.d. r.v.s

Let $X_1, X_2, \dots, X_n \stackrel{i.i.d.}{\sim} F$. The mgf of

$$Y := \sum_{i=1}^n X_i$$

is

$$M_Y(t) = [M_X(t)]^n.$$

Example 1.5.6

Suppose that $X_1, X_2, \dots, X_n \stackrel{i.i.d.}{\sim} \text{Poisson}(\lambda)$. Determine the distribution of $Y := \sum_{i=1}^n X_i$.

Example 1.5.6 (cont)

Example 1.5.6 (cont)

Example 1.5.7

Suppose that $X_1, X_2, \dots, X_n \stackrel{i.i.d.}{\sim} \text{Exponential}(\lambda)$. Determine the distribution of $Y := \sum_{i=1}^n X_i$.

Example 1.5.7 (cont)

Example 1.5.7 (cont)

Example 1.5.8

Suppose that X_1, X_2, \dots, X_n be independent random variables with $X_i \sim \text{Poisson}(\lambda_i)$. Determine the distribution of $Y := \sum_{i=1}^n X_i$.

Example 1.5.8 (cont)

Example 1.5.8 (cont)

Example 1.5.8 (cont)

1.6

General Order Statistics

1.6.2

The joint distribution of the minimum and maximum

Min/Max cdf

For an i.i.d. sample of continuous random variables X_1, X_2, \dots, X_n with cdf F , the joint cdf of $(X_{(1)}, X_{(n)})$ is

$$F_{X_{(1)}, X_{(n)}}(x, y) = [F(y)]^n - [F(y) - F(x)]^n,$$

for $x < y$ and

$$F_{X_{(1)}, X_{(n)}}(x, y) = [F(y)]^n$$

for $x \geq y$.

Proof of min/max cdf

Proof of min/max cdf (cont)

Proof of min/max cdf (cont)

Min/Max pdf

For an i.i.d. sample of continuous random variables X_1, X_2, \dots, X_n with cdf F , the joint pdf of $(X_{(1)}, X_{(n)})$ is

$$f_{X_{(1)}, X_{(n)}}(x, y) = n(n-1)[F(y) - F(x)]^{n-2} f(x)f(y),$$

for $x < y$.

Proof of min/max pdf

Example 1.6.1

Determine the joint pdf of $(X_{(1)}, X_{(15)})$ when $X_1, X_2, \dots, X_{15} \stackrel{i.i.d.}{\sim} \text{Uniform}(0, 1)$.

Example 1.6.1 (cont)

1.6.3

The distribution of all order statistics

PDF of all order statistics

For an i.i.d. sample of continuous random variables X_1, X_2, \dots, X_n with pdf f , the pdf of all n order statistics is

$$f_{X_{(1)}, X_{(2)}, \dots, X_{(n)}}(x_1, x_2, \dots, x_n) \\ = n! f(x_1) f(x_2) \cdots f(x_n) \underline{I(x_1 < x_2 < \cdots < x_{n-1} < x_n)}.$$

For $y_1 < x_1 \leq y_2 < x_2 < \cdots \leq y_n < x_n$

$$P(y_1 < X_{(1)} \leq x_1, y_2 < X_{(2)} \leq x_2, \dots, y_n < X_{(n)} \leq x_n) \\ = P(\{y_1 < X_1 \leq x_1, y_2 < X_2 \leq x_2, \dots, y_n < X_n \leq x_n\} \cup \\ \{y_1 < X_2 \leq x_1, y_2 < X_1 \leq x_2, y_3 < X_3 \leq x_3, \dots, y_n < X_n \leq x_n\} \cup \\ \vdots \\ n! \text{ permutations})$$

$$\begin{aligned}
\text{Proof} &= n! P(y_1 < X_1 \leq x_1, y_2 < X_2 \leq x_2, \dots, y_n < X_n \leq x_n) \\
&\stackrel{\text{ind.}}{=} n! P(y_1 < X_1 \leq x_1) P(y_2 < X_2 \leq x_2) \dots P(y_n < X_n \leq x_n) \\
&= n! \prod_{i=1}^n P(y_i < X_i \leq x_i) \\
&= n! \prod_{i=1}^n [F(x_i) - F(y_i)]
\end{aligned}$$

A simplified version of the first fundamental theorem of calc. is
 For $x \in [a, b]$, $\frac{d}{dx} \int_a^x f(t) dt = f(x)$.

$$\begin{aligned}
P(y_1 < X_{(1)} \leq x_1, \dots, y_n < X_{(n)} \leq x_n) &= \int_{y_n}^{x_n} \dots \int_{y_1}^{x_1} f_{X_{(1)}, \dots, X_{(n)}}(u_1, \dots, u_n) du_1 \dots du_n \Leftarrow \\
&= n! \prod_{i=1}^n [F(x_i) - F(y_i)] \Leftarrow
\end{aligned}$$

$$\begin{aligned}
\frac{d}{dx_n} \dots \frac{d}{dx_1} P(y_1 < X_{(1)} \leq x_1, \dots, y_n < X_{(n)} \leq x_n) &= \frac{d}{dx_n} \dots \frac{d}{dx_1} \int_{y_n}^{x_n} \dots \int_{y_1}^{x_1} f_{X_{(1)}, \dots, X_{(n)}}(u_1, \dots, u_n) du_1 \dots du_n \\
&= \frac{d}{dx_n} \dots \frac{d}{dx_1} n! \prod_{i=1}^n [F(x_i) - F(y_i)]
\end{aligned}$$

Proof Claim: $\frac{d}{dx_n} \dots \frac{d}{dx_1} n! \prod_{i=1}^n [F(x_i) - F(y_i)] = n! f(x_1) \dots f(x_n)$

For $n=1$, $\frac{d}{dx_1} \{ 1! [F(x_1) - F(y_1)] \} = 1! f(x_1) \checkmark$

For $n=2$, $\frac{d}{dx_2} \frac{d}{dx_1} \{ 2! [F(x_1) - F(y_1)] [F(x_2) - F(y_2)] \}$
 $\frac{d}{dx_2} \{ 2! f(x_1) [F(x_2) - F(y_1)] \}$
 $= 2! f(x_1) f(x_2) \checkmark$

Assume true for $n=k-1$, show for $n=k$

For $n=k$,
 $\frac{d}{dx_n} \dots \frac{d}{dx_1} n! \prod_{i=1}^n [F(x_i) - F(y_i)]$
 $= \frac{d}{dx_n} \dots \frac{d}{dx_1} n [F(x_n) - F(y_n)] (n-1)! \prod_{i=1}^{n-1} [F(x_i) - F(y_i)]$

$$= \frac{d}{dx_n} n [F(x_n) - F(y_n)] \left\{ \frac{d}{dx_{n-1}} \cdots \frac{d}{dx_1} (n-1)! \prod_{i=1}^{n-1} [F(x_i) - F(y_i)] \right\}$$

Proof

$$= \frac{d}{dx_n} n [F(x_n) - F(y_n)] \underbrace{(n-1)! f(x_1) \cdots f(x_{n-1})}_{f(x_n)}$$

$$= n(n-1)! f(x_n) f(x_1) \cdots f(x_{n-1})$$

$$= n! f(x_1) \cdots f(x_n) I(x_1 < x_2 < \cdots < x_n)$$

Proof

1.6.4

The distribution of $X_{(i)}$

CDF of $X_{(i)}$

For an i.i.d. sample of continuous random variables X_1, X_2, \dots, X_n with cdf F , the cdf of $X_{(i)}$ is

$$F_{X_{(i)}}(x) = P(X_{(i)} \leq x) = \sum_{j=i}^n \binom{n}{j} (1 - F(x))^{n-j} F(x)^j.$$

$$P(X_{(i)} \leq x) = P\left(\left\{X_{(n)} \leq x\right\} \cup \left\{X_{(n)} > x, X_{(n-1)} \leq x\right\} \cup \right. \\ \left. \vdots \right. \\ \left. \left\{X_{(n)} > x, X_{(n-1)} > x, \dots, X_{(i+1)} > x, X_{(i)} \leq x\right\}\right) \leftarrow \text{binomial}(n, F(x))$$

$$P(X_{(n)} > x, \dots, X_{(j+1)} > x, X_{(j)} \leq x) = \binom{n}{j} F(x)^j (1 - F(x))^{n-j}$$

$$\therefore F_{X_{(i)}}(x) = \sum_{j=i}^n \binom{n}{j} F(x)^j (1 - F(x))^{n-j}$$

Proof

Proof (cont)

The PDF of $X_{(i)}$

For an i.i.d. sample of continuous random variables X_1, X_2, \dots, X_n with cdf F , pdf of f the pdf of $X_{(i)}$ is

$$f_{X_{(i)}}(x) = \frac{n!}{(i-1)!(n-i)!} \underline{F(x)^{i-1}} \underline{(1-F(x))^{n-i}} \underline{f(x)}.$$

$$\begin{aligned} f_{X_{(i)}}(x) &= \frac{d}{dx} F_{X_{(i)}}(x) \Leftarrow \\ &= \frac{d}{dx} \sum_{j=i}^n \binom{n}{j} F(x)^j (1-F(x))^{n-j} \\ &= \sum_{j=i}^n \frac{d}{dx} \left\{ \binom{n}{j} F(x)^j [1-F(x)]^{n-j} \right\} \\ &= \sum_{j=i}^n \binom{n}{j} j [F(x)]^{j-1} f(x) [1-F(x)]^{n-j} \leftarrow \\ &\quad - \sum_{j=i}^n \binom{n}{j} F(x)^j \underline{(n-j)} (1-F(x))^{n-j-1} f(x) \end{aligned}$$

Proof

$$i \binom{n}{i} F(x)^{i-1} f(x) [1-F(x)]^{n-i}$$

$$+ \sum_{j=i+1}^n \binom{n}{j} j [F(x)]^{j-1} f(x) [1-F(x)]^{n-j} \leftarrow$$

$$- \sum_{j=i}^{n-1} \binom{n}{j} F(x)^j \underbrace{(n-j)}_{\rightarrow} [1-F(x)]^{n-j-1} f(x) \leftarrow$$

$$\text{Let } k = j-1$$

$$j \binom{n}{j} = j \frac{n!}{j! (n-j)!} = \frac{n!}{(j-1)! (n-j)!} = \frac{n!}{k! (n-k-1)!} = \frac{(n-k) n!}{k! (n-k)!} = (n-k) \binom{n}{k}$$

$$\sum_{k=i}^{n-1} (n-k) \binom{n}{k} F(x)^k \cancel{[1-F(x)]^{n-k-1}} f(x) \leftarrow$$

$$- \sum_{j=i}^{n-1} \underbrace{(n-j)}_{\rightarrow} \binom{n}{j} F(x)^j \cancel{[1-F(x)]^{n-j-1}} f(x) \leftarrow$$

Proof (cont)

$$f_{(i)}(x) = i \binom{n}{i} F(x)^{i-1} [1 - F(x)]^{n-i} f(x)$$

$$= i \frac{n!}{i! (n-i)!} F(x)^{i-1} [1 - F(x)]^{n-i} f(x)$$

$$= \frac{n!}{(i-1)! (n-i)!} F(x)^{i-1} [1 - F(x)]^{n-i} f(x)$$

$$= n \frac{(n-1)!}{(i-1)! (n-i)!} F(x)^{i-1} [1 - F(x)]^{n-i} f(x)$$

$$= n \binom{n-1}{i-1} F(x)^{i-1} [1 - F(x)]^{(n-1)-(i-1)}$$

Proof (cont)

1.6.5

The joint distribution of $X_{(i)}$ and $X_{(j)}$

The joint pdf of $X_{(i)}$ and $X_{(j)}$

For an i.i.d. sample of continuous random variables X_1, X_2, \dots, X_n with cdf F , the joint pdf of $(X_{(i)}, X_{(j)})$ is

$$\begin{aligned} & f_{X_{(i)}, X_{(j)}}(x_i, x_j) \\ &= \frac{n!}{(i-1)!(j-i-1)!(n-j)!} F(x_i)^{i-1} f(x_i) \\ & \quad \times [F(x_j) - F(x_i)]^{j-i-1} f(x_j) [1 - F(x_j)]^{n-j} I_{(-\infty, x_j)}(x_i). \end{aligned}$$